stuck

tree.v
@@ -1,3 +1,5 @@
+Require Import Coq.Numbers.Natural.Peano.NPeano.
+
 Inductive tree (X : Type) : Type :=
   | empty : tree X
   | node : X -> tree X -> tree X -> tree X.
@@ -25,27 +27,46 @@ Inductive non_empty {X : Type} : tree X -> Prop :=
 
 Inductive full {X : Type} : tree X -> Prop :=
   | full_empty : full empty
-  | full_leaf : forall x, full (node x empty empty)
+  | full_leaf : forall x, full (leaf x)
   | full_node : forall x l r,
       non_empty l -> full l ->
       non_empty r -> full r -> full (node x l r).
 
+Inductive perfect {X : Type} : tree X -> Prop :=
+  | perfect_empty : perfect empty
+  | perfect_leaf : forall x, perfect (leaf x)
+  | perfect_node : forall x l r,
+      non_empty l -> full l ->
+      non_empty r -> full r ->
+      size l = size r -> perfect (node x l r).
+
+Theorem perfect_implies_full : forall {X : Type} (t : tree X),
+  perfect t -> full t.
+Proof.
+  intros. induction H.
+    constructor. constructor. constructor.
+    auto. auto. auto. auto. 
+Qed.
+
+Theorem size_of_perfect : forall {X : Type} (t : tree X),
+  perfect t -> size t = 2 ^ (depth t) - 1.
+
 (** Tests **)
 
-Theorem test_full1: forall {X : Type}, full (empty : tree X).
+Theorem test_full1 : forall {X : Type}, full (empty : tree X).
 Proof. intros. apply full_empty. Qed.
 
-Theorem test_full2: full (leaf 1).
+Theorem test_full2 : full (leaf 1).
 Proof. intros. apply full_leaf. Qed.
 
-Theorem test_full3: full (node 1 (leaf 2) (leaf 3)).
+Theorem test_full3 : full (node 1 (leaf 2) (leaf 3)).
 Proof. intros. apply full_node.
  apply non_empty_node. apply full_leaf.
  apply non_empty_node. apply full_leaf.
 Qed.
 
-Example test_size1: size (node 0 empty (leaf 1)) = 2.
+Example test_size1 : size (node 0 empty (leaf 1)) = 2.
 Proof. reflexivity. Qed.
 
-Example test_depth1: depth (node 0 (node 2 empty empty) (node 1 empty empty)) = 2.
+Example test_depth1 : depth (node 0 (node 2 empty empty) (node 1 empty empty)) = 2.
 Proof. reflexivity. Qed.
